Complete Low* proof

01-long-subtraction/lowstar/LongSubtraction.fst
@@ -2,6 +2,7 @@ module LongSubtraction
 
 module B = LowStar.Buffer
 module HS = FStar.HyperStack
+module ST = FStar.HyperStack.ST
 module S = FStar.Seq
 
 open FStar.Mul
@@ -23,9 +24,31 @@ let v (h: HS.mem) (x: s) =
   UInt64.v (S.index words 2) * pow2 (64 * 2) +
   UInt64.v (S.index words 3) * pow2 (64 * 3)
 
+// The refinement type is convenient, but probably not essential.
 let borrow =
-  x:UInt64.t { UInt64.v x == 0 \/ UInt64.v x == 1 }
+  x:UInt8.t { UInt8.v x == 0 \/ UInt8.v x == 1 }
 
+// Subtraction with borrowing, on two u64s. This is a simplified version of the
+// standard signature that lives in HACL* (see Lib.IntTypes.Intrinsics.fsti and
+// Hacl.IntTypes.Intrinsics.fst). Here, for simplicity, we assume a modern
+// toolchain with support for the corresponding CPU intrinsic. The CPrologue
+// thing is kind of a hack but avoids having to write glue code by hand (and
+// allows asserting we got the signature right).
+[@@ CPrologue "#define LongSubtraction_sub_borrow _subborrow_u64"]
+assume val sub_borrow:
+  b_in:borrow ->
+  x: UInt64.t ->
+  y: UInt64.t ->
+  ret: B.pointer UInt64.t ->
+  Stack borrow
+    (requires fun h0 -> B.live h0 ret)
+    (ensures fun h0 b_out h1 ->
+      B.(modifies (loc_buffer ret) h0 h1) /\ (
+      let ret = B.deref h1 ret in
+      UInt64.v ret - UInt8.v b_out * pow2 64 == UInt64.v x - UInt64.v y - UInt8.v b_in))
+
+// The `Stack` annotation indicates that this function does not generate heap
+// allocations.
 val sub (dst x y: s) (b0: borrow): Stack borrow
   (requires fun h0 ->
     B.live h0 dst /\ B.live h0 x /\ B.live h0 y /\
@@ -34,4 +57,125 @@ val sub (dst x y: s) (b0: borrow): Stack borrow
     B.(loc_disjoint (loc_buffer dst) (loc_buffer x) \/ dst == x))
   (ensures fun h0 b1 h1 ->
     B.(modifies (loc_buffer dst) h0 h1) /\
-    v h1 dst - pow2 (64 * 4) * UInt64.v b1 == v h0 x - v h0 y - UInt64.v b0)
+    v h1 dst - pow2 (64 * 4) * UInt8.v b1 == v h0 x - v h0 y - UInt8.v b0)
+
+#set-options "--fuel 0 --ifuel 0 --z3rlimit 200"
+let sub dst x y b0 =
+  let h0 = ST.get () in
+
+  // Trick: trade reasoning about sequences for reasoning about disjointness.
+  let dst0 = B.sub dst 0ul 1ul in
+  let dst1 = B.sub dst 1ul 1ul in
+  let dst2 = B.sub dst 2ul 1ul in
+  let dst3 = B.sub dst 3ul 1ul in
+  assert B.(all_disjoint [ loc_buffer dst0; loc_buffer dst1; loc_buffer dst2; loc_buffer dst3 ]);
+
+  // Same deal here.
+  let x0 = B.sub x 0ul 1ul in
+  let x1 = B.sub x 1ul 1ul in
+  let x2 = B.sub x 2ul 1ul in
+  let x3 = B.sub x 3ul 1ul in
+  assert B.(all_disjoint [ loc_buffer x0; loc_buffer x1; loc_buffer x2; loc_buffer x3 ]);
+
+  // Not strictly necessary for the proof to go through, but helps make sure the
+  // solver and I are on the same page when it comes to the disjointness
+  // predicates in the presence of potential aliasing between `dst` and `x`
+  assert B.(all_disjoint [ loc_buffer dst0; loc_buffer x1; loc_buffer x2; loc_buffer x3 ]);
+  assert B.(all_disjoint [ loc_buffer x0; loc_buffer dst1; loc_buffer x2; loc_buffer x3 ]);
+  assert B.(all_disjoint [ loc_buffer x0; loc_buffer x1; loc_buffer dst2; loc_buffer x3 ]);
+  assert B.(all_disjoint [ loc_buffer x0; loc_buffer x1; loc_buffer x2; loc_buffer dst3 ]);
+
+  let open LowStar.BufferOps in
+
+  let b1 = sub_borrow b0 (!*x0) y.(0ul) dst0 in
+  let h1 = ST.get () in
+  assert (UInt64.v (B.get h1 dst 0) - UInt8.v b1 * pow2 64 ==
+    UInt64.v (B.get h0 x 0) - UInt64.v (B.get h0 y 0) - UInt8.v b0);
+  // This would be hella harder to prove without splitting x four-ways. I'm just
+  // reluctant to jump into sequence update index etc. Tried proving `B.get h1 x
+  // 1 == B.get h0 x 1` earlier and I struggled.
+  assert (B.deref h1 x1 == B.deref h0 x1);
+  assert (B.deref h1 x2 == B.deref h0 x2);
+  assert (B.deref h1 x3 == B.deref h0 x3);
+
+  let b2 = sub_borrow b1 (!*x1) y.(1ul) dst1 in
+  let h2 = ST.get () in
+  // Note that the assert is slightly more sophisticated since it refers to
+  // B.get h0 x 1 -- there are multiple hidden steps of reasoning here, such as:
+  // index 1 of x was not modified earlier, and deref x1 is the same as B.get x 1
+  assert (UInt64.v (B.get h2 dst 1) - UInt8.v b2 * pow2 64 ==
+    UInt64.v (B.get h0 x 1) - UInt64.v (B.get h0 y 1) - UInt8.v b1);
+  assert (B.get h2 dst 0 == B.get h1 dst 0);
+
+  let b3 = sub_borrow b2 (!*x2) y.(2ul) dst2 in
+  let h3 = ST.get () in
+  assert (UInt64.v (B.get h3 dst 2) - UInt8.v b3 * pow2 64 ==
+    UInt64.v (B.get h0 x 2) - UInt64.v (B.get h0 y 2) - UInt8.v b2);
+  // Framing (as opposed to sequence reasoning).
+  assert (B.get h3 dst 0 == B.get h1 dst 0);
+  assert (B.get h3 dst 1 == B.get h2 dst 1);
+
+  let b4 = sub_borrow b3 (!*x3) y.(3ul) dst3 in
+  let h4 = ST.get () in
+  assert (UInt64.v (B.get h4 dst 3) - UInt8.v b4 * pow2 64 ==
+    UInt64.v (B.get h0 x 3) - UInt64.v (B.get h0 y 3) - UInt8.v b3);
+  assert (B.get h4 dst 0 == B.get h1 dst 0);
+  assert (B.get h4 dst 1 == B.get h2 dst 1);
+  assert (B.get h4 dst 2 == B.get h3 dst 2);
+
+  // Now we can focus on the math proof /per se/, because we have made sure that
+  // the results are as we expect and that the aliasing / dynamic frames worked
+  // out properly. I like long calc chains -- low-key, easy to debug, easy to
+  // maintain.
+
+  calc (==) {
+    v h4 dst - pow2 (64 * 4) * UInt8.v b4;
+  (==) { }
+    UInt64.v (B.get h1 dst 0) +
+    UInt64.v (B.get h2 dst 1) * pow2 64 +
+    UInt64.v (B.get h3 dst 2) * pow2 (64 * 2) +
+    UInt64.v (B.get h4 dst 3) * pow2 (64 * 3) -
+    pow2 (64 * 4) * UInt8.v b4;
+  (==) { }
+    UInt8.v b1 * pow2 64 +
+    UInt64.v (B.get h0 x 0) - UInt64.v (B.get h0 y 0) - UInt8.v b0 +
+    (UInt8.v b2 * pow2 64 +
+    UInt64.v (B.get h0 x 1) - UInt64.v (B.get h0 y 1) - UInt8.v b1) * pow2 64 +
+    (UInt8.v b3 * pow2 64 +
+    UInt64.v (B.get h0 x 2) - UInt64.v (B.get h0 y 2) - UInt8.v b2) * pow2 (64 * 2) +
+    (UInt8.v b4 * pow2 64 +
+    UInt64.v (B.get h0 x 3) - UInt64.v (B.get h0 y 3) - UInt8.v b3) * pow2 (64 * 3) -
+    pow2 (64 * 4) * UInt8.v b4;
+  (==) { _ by (FStar.Tactics.Canon.canon ()) }
+    UInt8.v b1 * pow2 64 +
+    UInt64.v (B.get h0 x 0) - UInt64.v (B.get h0 y 0) +
+    UInt8.v b2 * pow2 64 * pow2 64 +
+      UInt64.v (B.get h0 x 1) * pow2 64 - UInt64.v (B.get h0 y 1) * pow2 64 - UInt8.v b1 * pow2 64 +
+    UInt8.v b3 * pow2 64 * pow2 (64 * 2) +
+    UInt64.v (B.get h0 x 2) * pow2 (64 * 2) - UInt64.v (B.get h0 y 2) * pow2 (64 * 2) - UInt8.v b2 * pow2 (64 * 2) +
+    UInt8.v b4 * pow2 64 * pow2 (64 * 3) +
+    UInt64.v (B.get h0 x 3) * pow2 (64 * 3) - UInt64.v (B.get h0 y 3) * pow2 (64 * 3) - UInt8.v b3 * pow2 (64 * 3) -
+    UInt8.v b4 * pow2 (64 * 4) // commute this term too
+    - UInt8.v b0;
+  (==) {
+    assert_norm (pow2 64 * pow2 64 == pow2 (64 * 2));
+    assert_norm (pow2 64 * pow2 (64 * 2) == pow2 (64 * 3));
+    assert_norm (pow2 64 * pow2 (64 * 3) == pow2 (64 * 4))
+  }
+    UInt8.v b1 * pow2 64 +
+    UInt64.v (B.get h0 x 0) - UInt64.v (B.get h0 y 0) +
+    UInt8.v b2 * pow2 (64 * 2) +
+      UInt64.v (B.get h0 x 1) * pow2 64 - UInt64.v (B.get h0 y 1) * pow2 64 - UInt8.v b1 * pow2 64 +
+    UInt8.v b3 * pow2 (64 * 3) +
+    UInt64.v (B.get h0 x 2) * pow2 (64 * 2) - UInt64.v (B.get h0 y 2) * pow2 (64 * 2) - UInt8.v b2 * pow2 (64 * 2) +
+    UInt8.v b4 * pow2 (64 * 4) +
+    UInt64.v (B.get h0 x 3) * pow2 (64 * 3) - UInt64.v (B.get h0 y 3) * pow2 (64 * 3) - UInt8.v b3 * pow2 (64 * 3) -
+    pow2 (64 * 4) * UInt8.v b4
+    - UInt8.v b0;
+  };
+
+  // Note: a much shorter, but imho less readable proof, would be to just have
+  // the three `assert_norm`s, followed by `assert (... the post-condition ...)
+  // by canon ()`.
+
+  b4
